ulib/FStar.Pervasives.fsti
@@ -720,6 +720,13 @@ val allow_informative_binders : unit
   *)
 val commute_nested_matches : unit
 
+(** This attribute controls extraction: it can be used to disable
+    extraction of a given top-level definition into a specific backend,
+    such as "OCaml". If any extracted code must call into an erased
+    function, an error will be raised (code 340).
+  *)
+val noextract_to (backend:string) : Tot unit
+
 ///  Controlling normalization
 
 (** In any invocation of the F* normalizer, every occurrence of
@@ -868,6 +875,3 @@ val with_type (#t: Type) (e: t) : Tot t
     One of its uses is in types of layered effect combinators that
     are subjected to stricter typing discipline (no subtyping) *)
 unfold let eqtype_as_type (a:eqtype) : Type = a
-
-irreducible
-let noextract_to (s:string) : unit = ()
